src/coq/dot/TODO.v
@@ -1,3 +1,11 @@
+Lemma invert_typing_sel: forall E t l T q s, E |== s -> (E, s) |= sel t l ~: T @ q ->   
+      exists T', exists q1, (E, s) |= t ~: T' @ q1 /\
+      exists DS, exists q2, (E, s) |= T' ~< DS @ q2 /\
+      exists D, lbl.binds l D DS /\
+      exists S, open_decl_cond D t (decl_tm S) /\
+      exists q3, (E, s) |= S ~<: T @ q3.
+Proof.
+
 Lemma subst_pres_typing : forall E x Tx t T v, 
   (exists q, ctx_bind E x Tx |= t ^^ x ~: T ^tp^ x @ q)
   -> value v 
@@ -17,22 +25,22 @@ Lemma invert_expands_concrete : forall E s Tc DS q, (E, s) |= Tc ~< DS @ q -> co
 Proof. Admitted.
 
 
-Lemma quality_soundness_sub : forall E DS DS' T U q1 q2, 
-  E |= T ~< DS @ precise -> 
-  E |= T ~<: U @ q1 -> 
-  E |= U ~< DS' @ q2 /\
-  E |= DS <:DS<: DS'.
-Proof. Admitted. 
-
 Theorem quality_soundness : forall E T DS DSp, 
   (exists q, E |= T ~< DS @ q) ->  E |= T ~< DSp @ precise -> E |= DSp <:DS<: DS.
 Proof. Admitted.
+  Lemma quality_soundness_sub : forall E DS DS' T U q1 q2, 
+    E |= T ~< DS @ precise -> 
+    E |= T ~<: U @ q1 -> 
+    E |= U ~< DS' @ q2 /\
+    E |= DS <:DS<: DS'.
+  Proof. Admitted. 
 
-Lemma invert_typing_lam : forall E S t U q s, E |== s -> (E, s) |= lam S t ~: U @ q -> 
-      exists q1, exists L, exists T, (forall x, x \notin L -> (ctx_bind (E, s) x S) |= (t ^^ x) ~: T @ q1) /\
-      wf_tp (E, s) (tp_fun S T) /\ lc_tp T /\
-      exists q2, (E, s) |= (tp_fun S T) ~<: U @ q2.
+
+Lemma invert_subtyping_top : 
+   (forall E q T DS, E |= T ~< DS @ q -> subsumes_top T -> DS = nil) /\
+   (forall E q T T', E |= T ~<: T' @ q -> subsumes_top T -> ~ has_tp_sel T' -> subsumes_top T').
 Proof. Admitted.
+
 
 Lemma invert_expands_fun: forall E S T DS q,  E |= tp_fun S T ~< DS @ q -> DS = nil.
 Proof. Admitted.
@@ -46,15 +54,11 @@ Lemma invert_subtyping_and_l : forall E T1 T2 T q, E |= tp_and T1 T2 ~<: T @ q -
   (exists q, E |= T1 ~<: T @ q) /\ (exists q, E |= T2 ~<: T @ q).
 Proof. Admitted.
 
-Lemma or_decls_nil_2 : forall ds1 ds2 ds, or_decls ds1 ds2 ds -> ds1 = nil \/ ds2 = nil -> ds = nil.
-Proof. Admitted.
 
-Lemma red_implies_peq: forall E s t t' s', E |== s' -> s |~ t ~~> t' ~| s' -> path t -> path t' -> path_eq (E, s') t t'. 
-Proof. Admitted.
-
-Lemma sub_decls_pres_binds : forall l D DS E DS' q,
-    LabelMapImpl.binds l D DS -> sub_decls E q DS' DS -> 
-      exists D', exists q, LabelMapImpl.binds l D' DS' /\ sub_decl E q D' D.
+Lemma invert_typing_lam : forall E S t U q s, E |== s -> (E, s) |= lam S t ~: U @ q -> 
+      exists q1, exists L, exists T, (forall x, x \notin L -> (ctx_bind (E, s) x S) |= (t ^^ x) ~: T @ q1) /\
+      wf_tp (E, s) (tp_fun S T) /\ lc_tp T /\
+      exists q2, (E, s) |= (tp_fun S T) ~<: U @ q2.
 Proof. Admitted.
 
 Lemma invert_typing_ref: forall E s a T q, (E, s) |= ref a ~: T @ q -> 
@@ -63,7 +67,7 @@ Lemma invert_typing_ref: forall E s a T q, (E, s) |= ref a ~: T @ q ->
 Proof. Admitted.
 
 
-Lemma inversion_red_store_dom : forall s t t' s', s |~ t ~~> t' ~| s' -> dom s [<=] dom s'.
+Lemma invert_red_store_dom : forall s t t' s', s |~ t ~~> t' ~| s' -> dom s [<=] dom s'.
 Proof. Admitted.
 
 
@@ -71,6 +75,16 @@ Lemma invert_wf_store_uniq : forall s, wf_store s -> uniq s.
 Proof. Admitted.
 
 
+Lemma or_decls_nil_2 : forall ds1 ds2 ds, or_decls ds1 ds2 ds -> ds1 = nil \/ ds2 = nil -> ds = nil.
+Proof. Admitted.
+
+Lemma red_implies_peq: forall E s t t' s', E |== s' -> s |~ t ~~> t' ~| s' -> path t -> path t' -> path_eq (E, s') t t'. 
+Proof. Admitted.
+
+Lemma sub_decls_pres_binds : forall l D DS E DS' q,
+    lbl.binds l D DS -> sub_decls E q DS' DS -> 
+      exists D', exists q, lbl.binds l D' DS' /\ sub_decl E q D' D.
+Proof. Admitted.
 
 
 Lemma sub_decls_monotone_or_2 : forall E DS DS' DX DX' DSX DSX', 
@@ -96,5 +110,5 @@ Lemma sub_decls_monotone_and : forall E DS DS' DX DSX DSX',
 Lemma open_lc_decl_ident: forall d t, lc_decl d -> open_decl_cond d t d. Proof. Admitted.
 Lemma open_lc_is_noop : forall T x, lc_tp T -> T = T ^tp^ x. Proof. Admitted.
 
-Lemma binds_map_3 : forall A B l v (f: A -> B) args, LabelMapImpl.binds l v ((LabelMapImpl.map f) args) -> exists v', LabelMapImpl.binds l v' args.
+Lemma binds_map_3 : forall A B l v (f: A -> B) args, lbl.binds l v ((lbl.map f) args) -> exists v', lbl.binds l v' args.
 Proof. Admitted.
