src/coq/dot/meta_decls.v
@@ -4,7 +4,7 @@ Require Import syntax_binding theory.
 Require Import Metatheory LibTactics_sf support.
 
 Lemma sub_decls_pres_binds : forall l D DS E DS' q,
-    LabelMapImpl.binds l D DS -> sub_decls E q DS' DS -> 
-      exists D', exists q, LabelMapImpl.binds l D' DS' /\ sub_decl E q D' D.
+    lbl.binds l D DS -> sub_decls E q DS' DS -> 
+      exists D', exists q, lbl.binds l D' DS' /\ sub_decl E q D' D.
 Proof. Admitted.
 
