src/coq/dot/support.v
@@ -4,5 +4,7 @@ Require Import Metatheory LibTactics_sf Labels.
 
 Ltac injsubst H := (injection H; intros; subst; clear H).
 
-Lemma binds_map_3 : forall A B l v (f: A -> B) args, LabelMapImpl.binds l v ((LabelMapImpl.map f) args) -> exists v', LabelMapImpl.binds l v' args.
+Module lbl := LabelMapImpl.
+
+Lemma binds_map_3 : forall A B l v (f: A -> B) args, lbl.binds l v ((lbl.map f) args) -> exists v', lbl.binds l v' args.
 Proof. Admitted.
